Lott/DSL/Parser.lean
@@ -43,18 +43,21 @@ syntax "metavar " ident,+ : command
 /- Non-terminal syntax. -/
 
 declare_syntax_cat Lott.Symbol
+declare_syntax_cat Lott.DSL.BindConfig
 declare_syntax_cat Lott.DSL.DesugarConfig
 declare_syntax_cat Lott.DSL.ElabConfig
 declare_syntax_cat Lott.DSL.Production
 declare_syntax_cat Lott.DSL.NonTerminal
 
+syntax "(" "bind" ident " in " ident,+ ")" : Lott.DSL.BindConfig
+
 syntax "(" "desugar" " := " term ")" : Lott.DSL.DesugarConfig
 
 syntax "(" "elab" " := " term ")" : Lott.DSL.ElabConfig
 
-syntax " | " stx+ " : " ident atomic(Lott.DSL.DesugarConfig)? (Lott.DSL.ElabConfig)? : Lott.DSL.Production
+syntax " | " stx+ " : " ident atomic(Lott.DSL.BindConfig)? atomic(Lott.DSL.DesugarConfig)? (Lott.DSL.ElabConfig)? : Lott.DSL.Production
 
-syntax "nonterminal " ("(" "parent" " := " ident ")")? ident,+ " := " Lott.DSL.Production* : Lott.DSL.NonTerminal
+syntax "nosubst"? "nonterminal " ("(" "parent" " := " ident ")")? ident,+ " := " Lott.DSL.Production* : Lott.DSL.NonTerminal
 
 syntax Lott.DSL.NonTerminal : command
 
